Capless/Subst/Type/Subtyping.lean
@@ -1,10 +1,35 @@
 import Capless.Subst.Basic
 import Capless.Subtyping
+import Capless.Subst.Type.Subcapturing
 namespace Capless
 
 theorem SSubtyp.tsubst
   (h : SSubtyp Γ S1 S2)
   (σ : TVarSubst Γ f Δ) :
   SSubtyp Δ (S1.trename f) (S2.trename f) := sorry
+
+theorem CSubtyp.tsubst
+  (h : CSubtyp Γ S1 S2)
+  (σ : TVarSubst Γ f Δ) :
+  CSubtyp Δ (S1.trename f) (S2.trename f) := by
+  cases h
+  case capt hc hs =>
+    simp [CType.trename]
+    apply CSubtyp.capt
+    { apply! Subcapt.tsubst }
+    { apply! SSubtyp.tsubst }
+
+theorem ESubtyp.tsubst
+  (h : ESubtyp Γ S1 S2)
+  (σ : TVarSubst Γ f Δ) :
+  ESubtyp Δ (S1.trename f) (S2.trename f) := sorry
+
+theorem ESubtyp.tnarrow
+  (h : ESubtyp (Γ.tvar (TBinding.bound S)) E1 E2)
+  (hs : SSubtyp Γ S' S) :
+  ESubtyp (Γ.tvar (TBinding.bound S')) E1 E2 := by
+  rw [<- EType.trename_id (E := E1), <- EType.trename_id (E := E2)]
+  apply? ESubtyp.tsubst
+  { apply? TVarSubst.narrow }
 
 end Capless
