Capless/Subst/Type/Typing.lean
@@ -7,4 +7,12 @@ theorem Typed.tsubst
   (σ : TVarSubst Γ f Δ) :
   Typed Δ (t.trename f) (E.trename f) := by sorry
 
+theorem Typed.tnarrow
+  (h : Typed (Γ.tvar (TBinding.bound S)) t E)
+  (hs : SSubtyp Γ S' S) :
+  Typed (Γ.tvar (TBinding.bound S')) t E := by
+  rw [<- Term.trename_id (t := t), <- EType.trename_id (E := E)]
+  apply? Typed.tsubst
+  apply? TVarSubst.narrow
+
 end Capless
