Capless/Type/Basic.lean
@@ -1,0 +1,8 @@
+import Capless.Type
+namespace Capless
+
+theorem SType.tvar_tweaken_succ :
+  (SType.tvar X : SType n m k).tweaken = SType.tvar X.succ := by
+  simp [SType.tweaken, SType.trename, FinFun.weaken]
+
+end Capless
